



ENGINEERING MATHEMATICS I

Kavyashree

Department of Science and
Humanities

Class content

Recurrence relations



Some important recurrence relations

1. $\frac{d}{dx} \left(x^n J_n(x) \right) = x^n J_{n-1}(x)$
2. $\frac{d}{dx} \left(x^{-n} J_n(x) \right) = -x^{-n} J_{n+1}(x)$
3. $\frac{d}{dx} J_n(x) = J_{n-1}(x) - \frac{n}{x} J_n(x)$
4. $\frac{d}{dx} J_n(x) = \frac{n}{x} J_n(x) - J_{n+1}(x)$
5. $\frac{d}{dx} J_n(x) = \frac{1}{2} \left(J_{n-1}(x) - J_{n+1}(x) \right)$
6. $2n J_n(x) = x \left(J_{n-1}(x) + J_{n+1}(x) \right)$

Recurrence relation 1

$$\frac{d}{dx} \left(x^n J_n(x) \right) = x^n J_{n-1}(x)$$

Proof: Consider $J_n(x) = \sum_{r=0}^{\infty} \frac{(-1)^r}{r! \Gamma(n+r+1)} \left(\frac{x}{2} \right)^{n+2r}$

Multiply by x^n on both sides, we get,

$$x^n J_n(x) = \sum_{r=0}^{\infty} \frac{(-1)^r x^n}{r! \Gamma(n+r+1)} \left(\frac{x}{2} \right)^{n+2r}$$

$$= \sum_{r=0}^{\infty} \frac{(-1)^r x^{2n+2r}}{r! \Gamma(n+r+1)} \left(\frac{1}{2} \right)^{n+2r}$$

Recurrence relation 1

Differentiating with respect to x, we get,

$$\begin{aligned}\frac{d}{dx}\left(x^n J_n(x)\right) &= \sum_{r=0}^{\infty} \frac{(-1)^r (2n+2r)x^{2n+2r-1}}{r!\Gamma(n+r+1)} \left(\frac{1}{2}\right)^{n+2r} \\ &= \sum_{r=0}^{\infty} \frac{(-1)^r (n+r)x^{2n+2r-1}}{r!\Gamma(n+r+1)2^{n+2r-1}} \\ &= \sum_{r=0}^{\infty} \frac{(-1)^r (n+r)x^n}{r!(n+r)\Gamma(n+r)} \left(\frac{x}{2}\right)^{n+2r-1}\end{aligned}$$

Recurrence relation 1

$$= x^n \sum_{r=0}^{\infty} \frac{(-1)^r (n+r)}{r! (n+r) \Gamma(n+r)} \left(\frac{x}{2} \right)^{n+2r-1}$$

$$= x^n J_{n-1}(x)$$

Thus,

$$\frac{d}{dx} \left(x^n J_n(x) \right) = x^n J_{n-1}(x)$$

Recurrence relation 2

$$\frac{d}{dx} \left(x^{-n} J_n(x) \right) = -x^{-n} J_{n+1}(x)$$

Proof: Consider $J_n(x) = \sum_{r=0}^{\infty} \frac{(-1)^r}{r! \Gamma(n+r+1)} \left(\frac{x}{2} \right)^{n+2r}$

Multiply by x^{-n} on both sides, we get,

$$x^{-n} J_n(x) = \sum_{r=0}^{\infty} \frac{(-1)^r x^{-n}}{r! \Gamma(n+r+1)} \left(\frac{x}{2} \right)^{n+2r}$$

Recurrence relation 2

$$= \sum_{r=0}^{\infty} \frac{(-1)^r x^{2r}}{r! \Gamma(n+r+1)} \left(\frac{1}{2}\right)^{n+2r}$$

Differentiating with respect to x, we get,

$$\frac{d}{dx} \left(x^{-n} J_n(x) \right) = \sum_{r=0}^{\infty} \frac{(-1)^r (2r) x^{2r-1}}{r! \Gamma(n+r+1)} \left(\frac{1}{2}\right)^{n+2r}$$

$$= \sum_{r=0}^{\infty} \frac{(-1)^r r x^{2r-1}}{r! \Gamma(n+r+1) 2^{n+2r-1}}$$

Recurrence relation 2

$$= \sum_{r=1}^{\infty} \frac{(-1)^r r x^{2r-1}}{r! \Gamma(n+r+1) 2^{n+2r-1}}$$

$$= \sum_{r=1}^{\infty} \frac{(-1)^r x^{2r-1}}{(r-1)! \Gamma(n+r+1) 2^{n+2r-1}}$$

$$= \sum_{r=1}^{\infty} \frac{(-1)^{(r-1+1)} x^{2(r-1+1)-1}}{(r-1)! \Gamma(n+r-1+1+1) 2^{n+2(r-1+1)-1}}$$

Recurrence relation 2

Put $s = r - 1$, then

$$\begin{aligned}\frac{d}{dx} \left(x^{-n} J_n(x) \right) &= \sum_{s=0}^{\infty} \frac{(-1)^{s+1} x^{2(s+1)-1}}{s! \Gamma(n+s+2) 2^{n+2(s+1)-1}} \\ &= -x^{-n} \sum_{s=0}^{\infty} \frac{(-1)^s x^{2s+(n+1)}}{s! \Gamma((n+1)+s+1) 2^{(n+1)+2s}} \\ &= -x^{-n} J_{n+1}(x)\end{aligned}$$

Thus $\frac{d}{dx} \left(x^{-n} J_n(x) \right) = -x^{-n} J_{n+1}(x)$

Recurrence relation 3

$$\frac{d}{dx} J_n(x) = J_{n-1}(x) - \frac{n}{x} J_n(x)$$

Proof: By recurrence relation 1

$$\frac{d}{dx} (x^n J_n(x)) = x^n J_{n-1}(x)$$

$$\Rightarrow x^n J_n'(x) + nx^{n-1} J_n(x) = x^n J_{n-1}(x)$$

$$\Rightarrow x^n \left\{ J_n'(x) + nx^{-1} J_n(x) \right\} = x^n J_{n-1}(x)$$

$$\Rightarrow J_n'(x) + \frac{n}{x} J_n(x) = J_{n-1}(x)$$

Thus

$$\frac{d}{dx} J_n(x) = J_{n-1}(x) - \frac{n}{x} J_n(x)$$

Recurrence relation 4

$$\frac{d}{dx} J_n(x) = \frac{n}{x} J_n(x) - J_{n+1}(x)$$

Proof: By recurrence relation 2

$$\frac{d}{dx} (x^{-n} J_n(x)) = -x^{-n} J_{n+1}(x)$$

$$\Rightarrow x^{-n} J_n'(x) - nx^{-n-1} J_n(x) = -x^{-n} J_{n+1}(x)$$

$$\Rightarrow x^{-n} \left\{ J_n'(x) - nx^{-1} J_n(x) \right\} = -x^{-n} J_{n+1}(x)$$

$$\Rightarrow J_n'(x) - \frac{n}{x} J_n(x) = -J_{n+1}(x)$$

Thus

$$\frac{d}{dx} J_n(x) = \frac{n}{x} J_n(x) - J_{n+1}(x)$$

Recurrence relation 5

$$\frac{d}{dx} J_n(x) = \frac{1}{2} (J_{n-1}(x) - J_{n+1}(x))$$

Proof: By recurrence relation 3

$$\frac{d}{dx} J_n(x) = J_{n-1}(x) - \frac{n}{x} J_n(x) \quad \text{--- --} \rightarrow (1)$$

By recurrence relation 4

$$\frac{d}{dx} J_n(x) = \frac{n}{x} J_n(x) - J_{n+1}(x) \quad \text{--- --} \rightarrow (2)$$

$$(1) + (2) \Rightarrow 2 \frac{d}{dx} J_n(x) = J_{n-1}(x) - J_{n+1}(x)$$

i.e. $\frac{d}{dx} J_n(x) = \frac{1}{2} (J_{n-1}(x) - J_{n+1}(x))$

Recurrence relation 5

$$2n J_n(x) = x(J_{n-1}(x) + J_{n+1}(x))$$

Proof: By recurrence relation 3

$$\frac{d}{dx} J_n(x) = J_{n-1}(x) - \frac{n}{x} J_n(x) \quad \text{--- -- --} \rightarrow (1)$$

By recurrence relation 4

$$\frac{d}{dx} J_n(x) = \frac{n}{x} J_n(x) - J_{n+1}(x) \quad \text{--- -- --} \rightarrow (2)$$

$$(1) - (2) \Rightarrow 0 = J_{n-1}(x) + J_{n+1}(x) - \frac{2n}{x} J_n(x)$$

i.e. $2n J_n(x) = x(J_{n-1}(x) + J_{n+1}(x))$



THANK YOU

Kavyashree

Department of Science and Humanities

Email:Kavyashree@pes.edu

Phone:9008455661; Extn:714